src/Trans2.v
@@ -15,14 +15,14 @@ Record t2state := T2St {
   T2SAltDisk: option storage  (* alternative disk for transactions, if in txn *)
 }.
 
-Inductive t2smstep : t2state -> t2state -> Prop :=
+Inductive t2step : t2state -> t2state -> Prop :=
   | T2smHalt: forall d oad,
-    t2smstep (T2St T2Halt d oad)                (T2St T2Halt d oad)
+    t2step (T2St T2Halt d oad)                (T2St T2Halt d oad)
   | T2smBegin: forall d rx,
-    t2smstep (T2St (T2Begin rx) d None)         (T2St rx d (Some d))
+    t2step (T2St (T2Begin rx) d None)         (T2St rx d (Some d))
   | T2smProg: forall d ad dp rx,
-    t2smstep (T2St (T2DProg dp rx) d (Some ad)) (T2St rx d (Some (drun dp ad)))
+    t2step (T2St (T2DProg dp rx) d (Some ad)) (T2St rx d (Some (drun dp ad)))
   | T2smCommit: forall d ad rx,
-    t2smstep (T2St (T2Commit rx) d (Some ad))   (T2St rx ad None)
+    t2step (T2St (T2Commit rx) d (Some ad))   (T2St rx ad None)
   | T2smAbort: forall d ad rx,
-    t2smstep (T2St (T2Abort rx) d (Some ad))    (T2St rx d None).
+    t2step (T2St (T2Abort rx) d (Some ad))    (T2St rx d None).
